\documentclass{article}
\input{../../preamble.tex}

\author{Truman E. Ellis}
\title{Time Stepping Notes}

\begin{document}
\maketitle

We wish to solve the system
\[
\frac{\partial U}{\partial t}+f(U)=0
\]

For a 6 stage ESDIRK algorithm, we have the Butcher Tableau:
\[
\begin{array}{c|cccccc}
  0 & 0 & 0 & 0 & 0 & 0 & 0 \\
  c_1 & a_{10} & a_{11} & 0 & 0 & 0 & 0 \\
  c_2 & a_{20} & a_{21} & a_{22} & 0 & 0 & 0 \\
  c_3 & a_{30} & a_{31} & a_{32} & a_{33} & 0 & 0 \\
  c_4 & a_{40} & a_{41} & a_{42} & a_{43} & a_{44} & 0 \\
  c_5 & a_{50} & a_{51} & a_{52} & a_{53} & a_{54} & a_{55} \\
  \hline
   & b_0 & b_1 & b_2 & b_3 & b_4 & b_5 \\
\end{array}
\]
For ESDIRK schemes, we enforce a ``stiffly accurate'' condition by requiring
that $a_{sj} = b_j$, where $s$ is the number of stages minus one. We also have
the condition that the final stage equals the value at the next time step. So
there is no reason to reassemble from the various stages.

We solve a series of equations for $k=0,\cdots,5$
\[
\frac{U^k}{a_{kk}\Delta t}+f(U^k)=\frac{U_n}{a_{kk}\Delta
t}-\sum_{j=0}^{k-1}\frac{a_{kj}}{a_{kk}}f(U^j)
\]
From the first equation we see that $U^0=U_n$. And we have that $U_{n+1}=U^s$.

For a nonlinear system, define residual
\[
R(U^k) =
\frac{U^k}{a_{kk}\Delta t}+f(U^k)-\frac{U_n}{a_{kk}\Delta
t}+\sum_{j=0}^{k-1}\frac{a_{kj}}{a_{kk}}f(U^j)
\]
Given an approximate solution $\tilde U^k$, we wish to solve for an increment
$\Delta U$ such that $U^k=\tilde U^k + \Delta U$ is a better approximation of
the exact solution. Approximating $R(U^k)$ by $R(\tilde U^k)+R'(\tilde
U^k)\Delta U=0$, we obtain a linearized equation
\[
\frac{\Delta U}{a_{kk}\Delta t}+f'(\tilde U^k)\Delta U
=\frac{U_n}{a_{kk}\Delta t}-\frac{\tilde U^k}{a_{kk}\Delta t}-f(\tilde U^k)
-\sum_{j=0}^{k-1}\frac{a_{kj}}{a_{kk}}f(U^j)
\]

For implicit Euler, this is just
\[
R(U)=\frac{U}{\Delta t}+f(U)-\frac{U_n}{\Delta t}
\]
\[
\frac{\Delta U}{\Delta t}+f'(\tilde U)\Delta U
=\frac{U_n}{\Delta t}-\frac{\tilde U}{\Delta t}
-f(\tilde U)
\]

\section*{Case Studies}
\subsection*{Convection-Diffusion}
\begin{align*}
  \frac{1}{\epsilon}\bfsigma-\Grad u&=0\\
  \frac{\partial u}{\partial t}+\Div(\bfbeta u-\bfsigma)-f&=0
\end{align*}
\begin{align*}
  \LRp{\frac{1}{\epsilon}\bfsigma,\bftau}+\LRp{u,\Div\bftau}-\LRa{\hat u,\tau_n}&=0\\
  \LRp{\frac{\partial u}{\partial t},v}-\LRp{\bfbeta u-\bfsigma,\Grad v}+\LRa{\hat f,v}-(f,v)&=0
\end{align*}
Here
\[
f(U)=\LRp{\frac{1}{\epsilon}\bfsigma,\bftau}+\LRp{u,\Div\bftau}-\LRa{\hat u,\tau_n}
-\LRp{\bfbeta u-\bfsigma,\Grad v}+\LRa{\hat f,v}-(f,v)
\]
But we choose not to split the traces and fluxes, so instead we have
\[
f(U)=\LRp{\frac{1}{\epsilon}\bfsigma,\bftau}+\LRp{u,\Div\bftau}
-\LRp{\bfbeta u-\bfsigma,\Grad v}-(f,v)
\]
while
\[
f'(U)=\LRp{\frac{1}{\epsilon}\bfsigma,\bftau}+\LRp{u,\Div\bftau}-\LRa{\hat u,\tau_n}
-\LRp{\bfbeta u-\bfsigma,\Grad v}+\LRa{\hat f,v}
\]
So, given initial solution $u_n$ and approximate solution $\tilde U=\{\tilde
u,\tilde\bfsigma\}$, we
arrive at a system
\begin{align*}
\frac{\delta u}{\Delta t}
+\LRp{\frac{1}{\epsilon}\delta\bfsigma,\bftau}
+\LRp{\delta u,\Div\bftau}-\LRa{\hat u,\tau_n}
-\LRp{\bfbeta \delta u-\delta\bfsigma,\Grad v}
+\LRa{\hat f,v}
\\=
\frac{u_n}{\Delta t}
+\frac{\tilde u}{\Delta t}
-\LRp{\frac{1}{\epsilon}\tilde\bfsigma,\bftau}
-\LRp{\tilde u,\Div\bftau}
+\LRp{\bfbeta \tilde u-\bfsigma,\Grad v}
+(f,v)
\end{align*}
If we let $\tilde U=0$, then $U_{n+1}=\tilde U+\delta U=\delta U$ and since
this is a linear equation, we arrive at
\begin{align*}
\frac{u}{\Delta t}
+\LRp{\frac{1}{\epsilon}\bfsigma,\bftau}
+\LRp{u,\Div\bftau}-\LRa{\hat u,\tau_n}
-\LRp{\bfbeta u-\bfsigma,\Grad v}
+\LRa{\hat f,v}
=
\frac{u_n}{\Delta t}
+(f,v)
\end{align*}
which is exactly our linear system.

\end{document}
