% -*- root: Dissertation.tex -*-
\documentclass[Dissertation.tex]{subfiles}
\begin{document}
\chapter{Comparison of Primitive, Conservation, and Entropy Variables for Compressible Navier-Stokes}
\label{sec:VariableComparison}
% \section{Nonlinear Formulation}
In this appendix we discuss some work we did exploring a comparison between three formulations of the 
compressible Navier-Stokes equations: primitive variables, conservation variables, and entropy variables.

\section{Primitive Variables}
We begin by recalling the definitions for primitive variables:
\begin{align*}
C_c&:=\rho\\
\bfC_m&:=\rho\bfu\\
C_e&:=\rho(C_v T+\frac{1}{2}\bfu\cdot\bfu)\\
\bfF_c&:=\rho\bfu\\
\mathbb{F}_m&:=\rho\bfu\otimes\bfu+\rho RT\bbI\\
\bfF_e&:=\rho\bfu\LRp{C_v T+\frac{1}{2}\bfu\cdot\bfu}+\bfu\rho RT\\
\bfK_c&:=\boldsymbol 0\\
\bbK_m&:=\LRp{\bbD+\bbD^T-\frac{2}{3}\trace(\bbD)\bbI}\\
\bfK_e&:=-\bfq+\bfu\cdot\LRp{\bbD+\bbD^T-\frac{2}{3}\trace(\bbD)\bbI}\\
\bbM_{\bbD}&:=\bbD\\
\bfM_{\bfq}&:=\frac{Pr}{C_p}\bfq\\
\bfG_{\bbD}&:=\bfu\\
G_{\bfq}&:=-T\,.
\end{align*}

\subsection{Linearized Terms}
Now we introduce the linearized terms:
\begin{align*}
\pd{C_c(\tilde W)}{W}\Delta W&:=
	\Delta\rho\\
\pd{\bfC_m(\tilde W)}{W}\Delta W&:=
	\Delta\rho\tilde\bfu+\tilde\rho\Delta\bfu\\
\pd{C_e(\tilde W)}{W}\Delta W&:=
	C_v\Delta\rho\tilde T+C_v\tilde\rho\Delta T
	+\frac{1}{2}\LRp{\Delta\rho\tilde\bfu\cdot\tilde\bfu+\tilde\rho\Delta\bfu\cdot\tilde\bfu+\tilde\rho\tilde\bfu\cdot\Delta\bfu}\\
\pd{\bfF_c(\tilde W)}{W}\Delta W&:=
	\Delta\rho\tilde\bfu+\tilde\rho\Delta\bfu\\
\pd{\mathbb{F}_m(\tilde W)}{W}\Delta W&:=
	\Delta\rho\tilde\bfu\otimes\tilde\bfu
	+\tilde\rho\Delta\bfu\otimes\tilde\bfu
	+\tilde\rho\tilde\bfu\otimes\Delta\bfu
	+R\LRp{\Delta\rho\tilde T+\tilde\rho\Delta T}\bbI\\
\pd{\bfF_e(\tilde W)}{W}\Delta W&:=
	C_v\Delta\rho\tilde\bfu\tilde T+C_v\tilde\rho\Delta\bfu\tilde T+C_v\tilde\rho\tilde\bfu\Delta T
	\\&\quad
	+\frac{1}{2}\Delta\rho\tilde\bfu\tilde\bfu\cdot\tilde\bfu
	+\frac{1}{2}\tilde\rho\Delta\bfu\tilde\bfu\cdot\tilde\bfu
	+\frac{1}{2}\tilde\rho\tilde\bfu\Delta\bfu\cdot\tilde\bfu
	+\frac{1}{2}\tilde\rho\tilde\bfu\tilde\bfu\cdot\Delta\bfu
	\\&\quad
	+R\Delta\bfu\tilde\rho\tilde T
	+R\tilde\bfu\Delta\rho\tilde T
	+R\tilde\bfu\tilde\rho\Delta T\\
\pd{\bfK_c(\tilde W)}{W}\Delta W&:=
	\boldsymbol 0\\
\pd{\bbK_m(\tilde W)}{W}\Delta W&:=
	\LRp{\Delta\bbD+\Delta\bbD^T-\frac{2}{3}\trace(\Delta\bbD)\bbI}\\
\pd{\bfK_e(\tilde W)}{W}\Delta W&:=
	-\Delta\bfq+\Delta\bfu\cdot\LRp{\tilde\bbD+\tilde\bbD^T-\frac{2}{3}\trace(\tilde\bbD)\bbI}
	\\&\quad
	+\tilde\bfu\cdot\LRp{\Delta\bbD+\Delta\bbD^T-\frac{2}{3}\trace(\Delta\bbD)\bbI}\\
\pd{\bbM_{\bbD}(\tilde W)}{W}\Delta W&:=
	\Delta\bbD\\
\pd{\bfM_{\bfq}(\tilde W)}{W}\Delta W&:=
	\frac{Pr}{C_p}\Delta\bfq\\
\pd{\bfG_{\bbD}(\tilde W)}{W}\Delta W&:=
	\Delta\bfu\\
\pd{G_{\bfq}(\tilde W)}{W}\Delta W&:=
	-\Delta T\,.
\end{align*}

\section{Conservation Variables}
Now we wish to do a change of variables to conservation variables: 
\begin{align*}
\rho&=\rho\\
\bfm&=\rho\bfu\\
E&=\rho\LRp{C_v T+\frac{1}{2}\bfu\cdot\bfu}
\end{align*}

\begin{align*}
C_c&:=\rho\\
\bfC_m&:=\bfm\\
C_e&:=E\\
\bfF_c&:=\bfm\\
\mathbb{F}_m&=\frac{\bfm\otimes\bfm}{\rho}+(\gamma-1)\LRp{E-\frac{\bfm\cdot\bfm}{2\rho}}\bbI\\
\bfF_e&=\gamma E\frac{\bfm}{\rho}-(\gamma-1)\frac{\bfm\cdot\bfm}{2\rho^2}\bfm\\
\bfK_c&:=\boldsymbol 0\\
\bbK_m&:=\LRp{\bbD+\bbD^T-\frac{2}{3}\trace(\bbD)\bbI}\\
\bfK_e&:=-\bfq+\frac{\bfm}{\rho}\cdot\LRp{\bbD+\bbD^T-\frac{2}{3}\trace(\bbD)\bbI}\\
\bbM_{\bbD}&:=\bbD\\
\bfM_{\bfq}&:=\frac{Pr}{C_p}\bfq\\
\bfG_{\bbD}&:=\frac{\bfm}{\rho}\\
G_{\bfq}&:=-\LRp{\frac{E-\frac{1}{2\rho}\bfm\cdot\bfm}{C_v\rho}}\,.
\end{align*}

\subsection{Linearized Terms}
\begin{align*}
\pd{C_c(\tilde W)}{W}\Delta W&:=
	\Delta\rho\\
\pd{\bfC_m(\tilde W)}{W}\Delta W&:=
	\Delta\bfm\\
\pd{C_e(\tilde W)}{W}\Delta W&:=
	\Delta E\\
\pd{\bfF_c(\tilde W)}{W}\Delta W&:=
	\Delta\bfm\\
\pd{\mathbb{F}_m(\tilde W)}{W}\Delta W&:=
	\frac{\Delta\bfm\otimes\tilde\bfm}{\tilde\rho}
	+\frac{\tilde\bfm\otimes\Delta\bfm}{\tilde\rho}
	-\frac{\tilde\bfm\otimes\tilde\bfm}{\tilde\rho^2}\Delta\rho
	\\&\quad
	+(\gamma-1)\LRp{\Delta E
	-\frac{\Delta\bfm\cdot\tilde\bfm}{2\tilde\rho}
	-\frac{\tilde\bfm\cdot\Delta\bfm}{2\tilde\rho}
	+\frac{\tilde\bfm\cdot\tilde\bfm}{2\tilde\rho^2}\Delta\rho
	}\bbI\\
\pd{\bfF_e(\tilde W)}{W}\Delta W&:=
	\gamma\LRp{
	\Delta E\frac{\tilde\bfm}{\tilde\rho}
	+\tilde E\frac{\Delta\bfm}{\tilde\rho}
	-\tilde E\frac{\tilde\bfm}{\tilde\rho^2}\Delta\rho}
	\\&\quad
	+(\gamma-1)\left(
	-\frac{\Delta\bfm\tilde\bfm\cdot\tilde\bfm}{2\tilde\rho^2}
	-\frac{\tilde\bfm\Delta\bfm\cdot\tilde\bfm}{2\tilde\rho^2}
	\right.\\&\quad\quad\left.
	-\frac{\tilde\bfm\tilde\bfm\cdot\Delta\bfm}{2\tilde\rho^2}
	+\frac{\tilde\bfm\tilde\bfm\cdot\tilde\bfm}{\tilde\rho^3}\Delta\rho\right)\\
\pd{\bfK_c(\tilde W)}{W}\Delta W&:=
	\boldsymbol 0\\
\pd{\bbK_m(\tilde W)}{W}\Delta W&:=
	\LRp{\Delta\bbD+\Delta\bbD^T-\frac{2}{3}\trace(\Delta\bbD)\bbI}\\
\pd{\bfK_e(\tilde W)}{W}\Delta W&:=
	-\Delta\bfq+\LRp{\frac{\Delta\bfm}{\tilde\rho}-\frac{\tilde\bfm}{\tilde\rho^2}\Delta\rho}
	\cdot\LRp{\tilde\bbD+\tilde\bbD^T-\frac{2}{3}\trace(\tilde\bbD)\bbI}
	\\&\quad
	+\frac{\tilde\bfm}{\tilde\rho}\cdot\LRp{\Delta\bbD+\Delta\bbD^T-\frac{2}{3}\trace(\Delta\bbD)\bbI}\\
\end{align*}
\begin{align*}
\pd{\bbM_{\bbD}(\tilde W)}{W}\Delta W&:=
	\Delta\bbD\\
\pd{\bfM_{\bfq}(\tilde W)}{W}\Delta W&:=
	\frac{Pr}{C_p}\Delta\bfq\\
\pd{\bfG_{\bbD}(\tilde W)}{W}\Delta W&:=
	\frac{\Delta\bfm}{\tilde\rho}-\frac{\tilde\bfm}{\tilde\rho^2}\Delta\rho\\
\pd{G_{\bfq}(\tilde W)}{W}\Delta W&:=
	-\left(\frac{\Delta E-\frac{1}{2\tilde\rho}\Delta\bfm\cdot\tilde\bfm
	-\frac{1}{2\tilde\rho}\tilde\bfm\cdot\Delta\bfm
	+\frac{1}{2\tilde\rho^2}\tilde\bfm\cdot\tilde\bfm\Delta\rho}{C_v\tilde\rho}
	\right.\\&\quad\left.
	-\frac{\tilde E-\frac{1}{2\tilde\rho}\tilde\bfm\cdot\tilde\bfm}{C_v\tilde\rho^2}\Delta\rho\right)
\,.
\end{align*}

\section{Entropy Variables}
Now we wish to do a change of variables to entropy variables:
\begin{align*}
V_c&=\frac{-E+(E-\frac{1}{2\rho}\bfm\cdot\bfm)\LRp{\gamma+1-\ln\LRs{\frac{(\gamma-1)(E-\frac{1}{2\rho}\bfm\cdot\bfm)}{\rho^\gamma}}}}
{E-\frac{1}{2\rho}\bfm\cdot\bfm}\\
\bfV_m&=\frac{\bfm}{E-\frac{1}{2\rho}\bfm\cdot\bfm}\\
V_e&=\frac{-\rho}{E-\frac{1}{2\rho}\bfm\cdot\bfm}\\
\end{align*}
with reverse mapping:
\begin{align*}
\rho&=-\alpha V_e\\
\bfm&=\alpha\bfV_m\\
E&=\alpha\LRp{1-\frac{1}{2V_e}\bfV_m\cdot\bfV_m}\\
\end{align*}
where 
\[
\alpha(V_c,\bfV_m,V_e)=\LRs{\frac{\gamma-1}{(-V_e)^\gamma}}^{\frac{1}{\gamma-1}}\exp\LRs{\frac{-\gamma+V_c-\frac{1}{2V_e}\bfV_m\cdot\bfV_m}{\gamma-1}}
\]

\begin{align*}
C_c&:=-\alpha V_e\\
\bfC_m&:=\alpha\bfV_m\\
C_e&:=\alpha\LRp{1-\frac{1}{2V_e}\bfV_m\cdot\bfV_m}\\
\bfF_c&=\alpha\bfV_m\\
\mathbb{F}_m&=\alpha\LRp{-\frac{\bfV_m\otimes\bfV_m}{V_e}+(\gamma-1)\bbI}\\
\bfF_e&=\alpha\frac{\bfV_m}{V_e}\LRp{\frac{1}{2V_e}\bfV_m\cdot\bfV_m-\gamma}\\
\bfK_c&:=\boldsymbol 0\\
\bbK_m&:=\LRp{\bbD+\bbD^T-\frac{2}{3}\trace(\bbD)\bbI}\\
\bfK_e&:=-\bfq+\frac{\bfV_m}{V_e}\cdot\LRp{\bbD+\bbD^T-\frac{2}{3}\trace(\bbD)\bbI}\\
\bbM_{\bbD}&:=\bbD\\
\bfM_{\bfq}&:=\frac{Pr}{C_p}\bfq\\
\bfG_{\bbD}&:=\frac{\bfV_m}{V_e}\\
G_{\bfq}&:=\frac{1}{C_vV_e}\,.
\end{align*}

\subsection{Linearized Terms}
\begin{align*}
\pd{C_c(\tilde W)}{W}\Delta W&:=
	\Delta\rho
	\\
\pd{\bfC_m(\tilde W)}{W}\Delta W&:=
	\Delta\rho\tilde\bfu+\tilde\rho\Delta\bfu
	\\
\pd{C_e(\tilde W)}{W}\Delta W&:=
	C_v\Delta\rho\tilde T+C_v\tilde\rho\Delta T
	+\frac{1}{2}\LRp{\Delta\rho\tilde\bfu\cdot\tilde\bfu+\tilde\rho\Delta\bfu\cdot\tilde\bfu+\tilde\rho\tilde\bfu\cdot\Delta\bfu}
	\\
\pd{\bfF_c(\tilde W)}{W}\Delta W&:=
	\Delta\rho\tilde\bfu+\tilde\rho\Delta\bfu
	\\
\pd{\mathbb{F}_m(\tilde W)}{W}\Delta W&:=
	\Delta\rho\tilde\bfu\otimes\tilde\bfu
	+\tilde\rho\Delta\bfu\otimes\tilde\bfu
	+\tilde\rho\tilde\bfu\otimes\Delta\bfu
	+R\LRp{\Delta\rho\tilde T+\tilde\rho\Delta T}\bbI
	\\
\pd{\bfF_e(\tilde W)}{W}\Delta W&:=
	C_v\Delta\rho\tilde\bfu\tilde T+C_v\tilde\rho\Delta\bfu\tilde T+C_v\tilde\rho\tilde\bfu\Delta T
	\\&\quad
	+\frac{1}{2}\Delta\rho\tilde\bfu\tilde\bfu\cdot\tilde\bfu
	+\frac{1}{2}\tilde\rho\Delta\bfu\tilde\bfu\cdot\tilde\bfu
	+\frac{1}{2}\tilde\rho\tilde\bfu\Delta\bfu\cdot\tilde\bfu
	+\frac{1}{2}\tilde\rho\tilde\bfu\tilde\bfu\cdot\Delta\bfu
	\\&\quad
	+R\Delta\bfu\tilde\rho\tilde T
	+R\tilde\bfu\Delta\rho\tilde T
	+R\tilde\bfu\tilde\rho\Delta T
	\\
\pd{\bfK_c(\tilde W)}{W}\Delta W&:=
	\boldsymbol 0\\
\pd{\bbK_m(\tilde W)}{W}\Delta W&:=
	\LRp{\Delta\bbD+\Delta\bbD^T-\frac{2}{3}\trace(\Delta\bbD)\bbI}
	\\
\pd{\bfK_e(\tilde W)}{W}\Delta W&:=
	-\Delta\bfq+\Delta\bfu\cdot\LRp{\tilde\bbD+\tilde\bbD^T-\frac{2}{3}\trace(\tilde\bbD)\bbI}
	\\&\quad
	+\tilde\bfu\cdot\LRp{\Delta\bbD+\Delta\bbD^T-\frac{2}{3}\trace(\Delta\bbD)\bbI}\\
\pd{\bbM_{\bbD}(\tilde W)}{W}\Delta W&:=
	\Delta\bbD
	\\
\pd{\bfM_{\bfq}(\tilde W)}{W}\Delta W&:=
	\frac{Pr}{C_p}\Delta\bfq
	\\
\pd{\bfG_{\bbD}(\tilde W)}{W}\Delta W&:=
	\Delta\bfu
	\\
\pd{G_{\bfq}(\tilde W)}{W}\Delta W&:=
	-\Delta T
	\,.
\end{align*}

\end{document}
